move Exit from grove_ffi to machine

src/goose_lang/lib/control/impl.v
@@ -15,4 +15,9 @@ Definition Assert: val :=
   λ: "cond", if: Var "cond" then #()
              else Panic "assert failed".
 
+(** [Exit n] is supposed to exit the process. We cannot directly model
+this 9in GooseLang, so we just loop. *)
+Definition Exit: val :=
+  λ: <>, (rec: "loop" <> := Var "loop" #()) #().
+
 End goose_lang.
